DLCF/Typing/Basic.lean
@@ -9,217 +9,198 @@ def imax (n : ℕ) : ℕ → ℕ
 namespace Term
 
 inductive JEq : Finset FVar → Term → Term → Term → Prop
-  | nil_ok : JEq ∅ ⊤ .nil .nil
-  | cons_ok (hA : JEq Γ (.univ n) A A) : JEq (insert ⟨i, A⟩ Γ) ⊤ .nil .nil
+  -- Congruence
+  | top_emp : JEq ∅ (.univ 0) ⊤ ⊤
+  | top_cons (hA : JEq Γ (.univ n) A A) : JEq (insert ⟨i, A⟩ Γ) (.univ 0) ⊤ ⊤
   | var (hΓ : JEq Γ (.univ n) A A) (hx : ⟨i, A⟩ ∈ Γ) : JEq Γ A (.free i A) (.free i A)
-  | top (hΓ : JEq Γ ⊤ .nil .nil) : JEq Γ (.univ 0) .top .top
-  | bot (hΓ : JEq Γ ⊤ .nil .nil) : JEq Γ (.univ 0) .bot .bot
-  | univ (hΓ : JEq Γ ⊤ .nil .nil) : JEq Γ (.univ (n + 1)) (.univ n) (.univ n)
-  -- TODO: swap from cofinite quantification to universal?
-  | pi
+  | bot (hΓ : JEq Γ (.univ 0) ⊤ ⊤) : JEq Γ (.univ 0) ⊥ ⊥
+  | tt (hΓ : JEq Γ (.univ 0) ⊤ ⊤) : JEq Γ ⊤ (.epsilon ⊤) (.epsilon ⊤)
+  | univ (hΓ : JEq Γ (.univ 0) ⊤ ⊤) : JEq Γ (.univ (n + 1)) (.univ n) (.univ n)
+  | trunc (hΓ : JEq Γ (.univ n) A B) : JEq Γ (.univ 0) (.trunc A) (.trunc B)
+  | dite (hφ : JEq Γ (.univ 0) φ φ') (ht : JEq Γ A t t') (hf : JEq Γ A f f')
+    : JEq Γ A (.dite φ t f) (.dite φ' t' f')
+  | pi (hA : JEq Γ (.univ n) A A') (L : Finset ℕ)
+    (h : ∀i ∉ L, JEq (insert ⟨i, A⟩ Γ) (.univ m)
+    (B.bsubst (Term.free i A).b0)
+    (B'.bsubst (Term.free i A).b0))
+    : JEq Γ (.univ (n ⊔ m ⊔ 1)) (.pi A B) (.pi A' B')
+  | abs (hA : JEq Γ (.univ n) A A') (L : Finset ℕ)
+    (h : ∀i ∉ L, JEq (insert ⟨i, A⟩ Γ) (B.bsubst (Term.free i A).b0)
+    (b.bsubst (Term.free i A).b0)
+    (b'.bsubst (Term.free i A).b0))
+    : JEq Γ (.pi A B) (.abs A b) (.abs A' b')
+  | app (hf : JEq Γ (.pi A B) f f') (ha : JEq Γ A a a')
+    : JEq Γ (B.bsubst a.b0) (.app f a) (.app f' a')
+  -- Reduction rules
+  | dite_top (ht : JEq Γ A t t') (hf : JEq Γ A f f') : JEq Γ A (.dite ⊤ t f) t'
+  | dite_bot (ht : JEq Γ A t t') (hf : JEq Γ A f f') : JEq Γ A (.dite ⊥ t f) f'
+  | β_abs {a A b B : Term}
     (hA : JEq Γ (.univ n) A A')
-    (hx : ⟨i, A⟩ ∉ Γ ∪ fv B)
-    (hB : JEq (insert ⟨i, A⟩ Γ) (.univ m) (b0 (.free i A) • B) (b0 (.free i A) • B'))
-    : JEq Γ (.univ (imax n m)) (.pi A B) (.pi A' B')
-  | app (hf : JEq Γ (.pi A B) f f') (ha : JEq Γ A a a') : JEq Γ (b0 a • B) (.app f a) (.app f' a')
-  | abs
-    (hA : JEq Γ (.univ n) A A')
-    (hx : ⟨i, A⟩ ∉ Γ ∪ fv t)
-    (ht : JEq (insert ⟨i, A⟩ Γ) (b0 (.free i A) • B) (b0 (.free i A) • t) (b0 (.free i A) • t'))
-    : JEq Γ (.pi A B) (.abs A t) (.abs A' t')
-  | eq
-    (hA : JEq Γ (.univ n) A A')
+    (L : Finset ℕ)
+    (h : ∀i ∉ L, JEq (insert ⟨i, A⟩ Γ) (B.bsubst (Term.free i A).b0)
+    (b.bsubst (Term.free i A).b0)
+    (b.bsubst (Term.free i A).b0))
     (ha : JEq Γ A a a')
-    (hb : JEq Γ A b b')
-    : JEq Γ (.univ 0) (.eq A a b) (.eq A' a' b')
-  | eq_rfl (jab : JEq Γ A a b) : JEq Γ (.eq A a b) .nil .nil
-  -- β-reduction
-  | β_abs
-    (h : JEq Γ B l (.app (.abs A t) r)) : JEq Γ B l (b0 r • t)
-  -- η-expansion
-  | η_abs (h : JEq Γ (.pi A B) l r) : JEq Γ (.pi A B) l (.abs A (.app r (.bound 0)))
-  -- Extensionality
-  | jeq_ext (eab : JEq Γ (.eq A a b) .nil .nil) : JEq Γ A a b
-  -- Propositional extensionality
-  | u0_ext
-    (hA : JEq Γ (.univ 0) A A)
-    (hB : JEq Γ (.univ 0) B B)
-    (hAB : JEq Γ (.arr A B) .nil .nil)
-    (hBA : JEq Γ (.arr B A) .nil .nil)
+    : JEq Γ (B.bsubst a.b0) (.app (.abs A b) a) (b.bsubst a.b0)
+  -- Axioms
+  | pr_ext (hA : JEq Γ (.univ 0) A A') (hB : JEq Γ (.univ 0) B B')
+    (hf : JEq Γ (.arr A B) f f') (hg : JEq Γ (.arr B A) g g')
     : JEq Γ (.univ 0) A B
-  -- Propositional irrelevance
-  | u0_irr (hA : JEq Γ (.univ 0) A A) (ha : JEq Γ A a a) : JEq Γ A a .nil
-  -- Double negation elimination
-  -- TODO: generalize to truncation elimination
-  | dne (hA : JEq Γ (.univ 0) A A) (hna : JEq Γ (.neg (.neg A)) .nil .nil) : JEq Γ A .nil .nil
-  -- The axiom of choice
-  | aoc (hf : JEq Γ (.pi A (.trunc B)) .nil .nil) : JEq Γ (.trunc (.pi A B)) .nil .nil
-  | symm : JEq Γ A a b → JEq Γ A b a
-  | cast : JEq Γ (.univ n) A B → JEq Γ A a b → JEq Γ B a b
-  | trans : JEq Γ A a b → JEq Γ A b c → JEq Γ A a c
+  -- Casting
+  | cast (h : JEq Γ (.univ n) A B) (hab : JEq Γ A a b) : JEq Γ B a b
+  -- Partial equivalence
+  | trans (hab : JEq Γ A a b) (hbc : JEq Γ B b c) : JEq Γ A a c
+  | symm (hab : JEq Γ A a b) : JEq Γ A b a
 
-attribute [simp] JEq.nil_ok
+attribute [simp] JEq.top_emp
 
 notation Γ " ⊢ " a " ≡ " b " : " A => JEq Γ A a b
 
-theorem JEq.to_nil (h : Γ ⊢ a ≡ b : A) : Γ ⊢ .nil ≡ .nil : ⊤ := by induction h with
-  | nil_ok => exact .nil_ok
-  | cons_ok hA => exact .cons_ok hA
+theorem JEq.to_top (h : Γ ⊢ a ≡ b : A) : Γ ⊢ ⊤ ≡ ⊤ : .univ 0 := by induction h with
+  | top_emp => exact .top_emp
+  | top_cons hA => exact .top_cons hA
   | _ => assumption
 
--- notation Γ " ok" => Γ ⊢ Term.nil : ⊤
+theorem JEq.left_refl_jeq (h : Γ ⊢ a ≡ b : A) : Γ ⊢ a ≡ a : A := .trans h (.symm h)
+
+theorem JEq.right_refl_jeq (h : Γ ⊢ a ≡ b : A) : Γ ⊢ b ≡ b : A := .trans (.symm h) h
+
+def Ok (Γ : Finset FVar) : Prop := ∃a b A, Γ ⊢ a ≡ b : A
+
+theorem JEq.ok (h : Γ ⊢ a ≡ b : A) : Ok Γ := ⟨_, _, _, h⟩
+
+theorem JEq.ok_var (h : Γ ⊢ A ≡ A' : .univ n) (i) : Ok (insert ⟨i, A⟩ Γ)
+  := ⟨_, _, _, .top_cons h.left_refl_jeq⟩
+
+theorem Ok.top (h : Ok Γ) : Γ ⊢ ⊤ ≡ ⊤ : .univ 0 := by have ⟨_, _, _, h⟩ := h; exact h.to_top
+
+@[simp]
+theorem JEq.top_iff : (Γ ⊢ ⊤ ≡ ⊤ : .univ 0) ↔ Ok Γ := ⟨JEq.ok, Ok.top⟩
+
+theorem Ok.bot (h : Ok Γ) : Γ ⊢ ⊥ ≡ ⊥ : .univ 0 := .bot h.top
+
+@[simp]
+theorem JEq.bot_iff : (Γ ⊢ ⊥ ≡ ⊥ : .univ 0) ↔ Ok Γ := ⟨JEq.ok, Ok.bot⟩
+
+theorem Ok.tt (h : Ok Γ) : Γ ⊢ .epsilon ⊤ ≡ .epsilon ⊤ : ⊤ := .tt h.top
+
+@[simp]
+theorem JEq.tt_iff : (Γ ⊢ .epsilon ⊤ ≡ .epsilon ⊤ : ⊤) ↔ Ok Γ := ⟨JEq.ok, Ok.tt⟩
+
+theorem Ok.univ (h : Ok Γ) : Γ ⊢ .univ n ≡ .univ n : .univ (n + 1) := .univ h.top
+
+@[simp]
+theorem JEq.univ_iff : (Γ ⊢ .univ n ≡ .univ n : .univ (n + 1)) ↔ Ok Γ := ⟨JEq.ok, Ok.univ⟩
+
+theorem JEq.wk (hΔ : Ok Δ) (w : Γ ⊆ Δ) (h : Γ ⊢ a ≡ b : A) : Δ ⊢ a ≡ b : A
+  := by induction h generalizing Δ with
+  | top_emp | top_cons => exact hΔ.top
+  | trans hab hbc Iab Ibc => exact .trans (Iab hΔ w) (Ibc hΔ w)
+  | symm hab I => exact .symm (I hΔ w)
+  | _ => constructor
+    <;> intros
+    <;> (repeat first
+    | assumption
+    | apply JEq.ok_var
+    | apply Finset.insert_subset_insert
+    | apply_assumption)
+
+theorem JEq.wki (h : Γ ⊢ a ≡ b : A) (hB : Γ ⊢ B ≡ B' : .univ n): insert ⟨i, B⟩ Γ ⊢ a ≡ b : A
+  := h.wk (hB.ok_var i) (by simp)
+
+theorem JEq.arr (hA : Γ ⊢ A ≡ A' : .univ n) (hB : Γ ⊢ B ≡ B' : .univ m)
+  : Γ ⊢ .arr A B ≡ .arr A' B' : .univ (n ⊔ m ⊔ 1) := by
+  apply JEq.pi hA ∅
+  intro i
+  simp only [Finset.not_mem_empty, not_false_eq_true, bsubst0_wk0, forall_const]
+  apply hB.wki hA
+
+theorem JEq.mem_exists (h : Γ ⊢ a ≡ b : A) (hx : ⟨i, B⟩ ∈ Γ)
+  : ∃n, Γ ⊢ B ≡ B : .univ n := by induction h with
+  | top_emp => cases hx
+  | top_cons hA IA =>
+    simp only [Finset.mem_insert, FVar.mk.injEq] at hx
+    cases hx with
+    | inl hx => cases hx.1; cases hx.2; exact ⟨_, hA.wki hA⟩
+    | inr hx => have ⟨n, IA⟩ := IA hx; exact ⟨n, IA.wki hA⟩
+  | _ => apply_assumption; assumption
+
+theorem Ok.mem_exists (h : Ok Γ) (hA : ⟨i, A⟩ ∈ Γ) : ∃n, Γ ⊢ A ≡ A : .univ n := h.top.mem_exists hA
+
+theorem Ok.var (h : Ok Γ) (hx : ⟨i, A⟩ ∈ Γ) : Γ ⊢ .free i A ≡ .free i A : A
+  := have ⟨_, hA⟩ := h.mem_exists hx; .var hA hx
+
+inductive OkL : List FVar → Prop
+  | nil : OkL []
+  | cons (hA : Γ.toFinset ⊢ A ≡ A : .univ n) (hΓ : OkL Γ) : OkL (⟨i, A⟩ :: Γ)
+
 
 inductive HasTy : Finset FVar → Term → Term → Prop
-  | nil_ok : HasTy ∅ ⊤ .nil
-  | cons_ok (hA : HasTy Γ (.univ n) A) : HasTy (insert ⟨i, A⟩ Γ) ⊤ .nil
-  | var (hΓ : HasTy Γ (.univ n) A) (hx : ⟨i, A⟩ ∈ Γ) : HasTy Γ A (.free i A)
-  | top (hΓ : HasTy Γ ⊤ .nil) : HasTy Γ (.univ 0) ⊤
-  | bot (hΓ : HasTy Γ ⊤ .nil) : HasTy Γ (.univ 0) .bot
-  | univ (hΓ : HasTy Γ ⊤ .nil) : HasTy Γ (.univ (n + 1)) (.univ n)
-  | pi
-    (hA : HasTy Γ (.univ n) A)
-    (hx : ⟨i, A⟩ ∉ Γ ∪ fv B)
-    (hB : HasTy (insert ⟨i, A⟩ Γ) (.univ m) (b0 (.free i A) • B))
-    : HasTy Γ (.univ (imax n m)) (.pi A B)
-  | app (hf : HasTy Γ (.pi A B) f) (ha : HasTy Γ A a) : HasTy Γ (b0 a • B) (.app f a)
-  | abs
-    (hA : HasTy Γ (.univ n) A)
-    (hx : ⟨i, A⟩ ∉ Γ ∪ fv t)
-    (ht : HasTy (insert ⟨i, A⟩ Γ) (b0 (.free i A) • B) (b0 (.free i A) • t))
-    : HasTy Γ (.pi A B) (.abs A t)
-  | eq
-    (hA : HasTy Γ (.univ n) A)
-    (ha : HasTy Γ A a)
-    (hb : HasTy Γ A b)
-    : HasTy Γ (.univ 0) (.eq A a b)
-  | eq_rfl (h : Γ ⊢ a ≡ b : A) : HasTy Γ (.eq A a b) .nil
+  | var (hΓ : Ok Γ) (hx : ⟨i, A⟩ ∈ Γ) : HasTy Γ A (.free i A)
+  | top (hΓ : Ok Γ) : HasTy Γ (.univ 0) ⊤
+  | bot (hΓ : Ok Γ) : HasTy Γ (.univ 0) ⊥
+  | tt (hΓ : Ok Γ) : HasTy Γ ⊤ (.epsilon ⊤)
+  | univ (hΓ : Ok Γ) : HasTy Γ (.univ (n + 1)) (.univ n)
+  | dite (hφ : HasTy Γ (.univ 0) φ) (ht : HasTy Γ A t) (hf : HasTy Γ A f)
+    : HasTy Γ A (.dite φ t f)
+  | pi (hA : HasTy Γ (.univ n) A) (L : Finset ℕ)
+    (hB : ∀i ∉ L, HasTy (insert ⟨i, A⟩ Γ) (.univ m) (B.bsubst (Term.free i A).b0))
+    : HasTy Γ (.univ (n ⊔ m ⊔ 1)) (.pi A B)
   | cast (h : Γ ⊢ A ≡ B : .univ n) (ha : HasTy Γ A a) : HasTy Γ B a
 
 notation Γ " ⊢ " a " : " A => HasTy Γ A a
 
-theorem HasTy.refl {Γ A a} (h : Γ ⊢ a : A) : Γ ⊢ a ≡ a : A := by induction h with
+theorem HasTy.ok (h : Γ ⊢ a : A) : Ok Γ := by induction h with
+  | _ => assumption
+
+theorem HasTy.refl (h : Γ ⊢ a : A) : Γ ⊢ a ≡ a : A := by induction h with
+  | top hΓ => exact hΓ.top
+  | var hΓ hx => exact hΓ.var hx
   | cast h ha Ia => exact .cast h Ia
-  | _ => constructor <;> (try apply JEq.to_nil) <;> assumption
+  | _ => constructor <;> (try apply Ok.top) <;> assumption
 
--- theorem JEq.left_eq_helper {Γ A a} (h : Γ ⊢ a ≡ b : A) (hab : a = b) : Γ ⊢ a : A := by
---   induction h with
---   | β_abs => sorry -- TODO: needs inversion + substitution
---   | η_abs => sorry
---   | jeq_ext => sorry
---   | u0_ext => sorry
---   | u0_irr => sorry
---   | dne => sorry
---   | aoc => sorry
---   | symm => sorry
---   | cast => sorry
---   | trans => sorry
---   | _ => cases hab; constructor <;> apply_assumption <;> rfl
+theorem HasTy.ok_var (h : Γ ⊢ A : .univ n) (i) : Ok (insert ⟨i, A⟩ Γ) := h.refl.ok_var i
 
--- theorem JEq.left {Γ A a} (h : Γ ⊢ a ≡ b : A) : Γ ⊢ a : A := by
-  -- induction h with
-  -- | pi => sorry
-  -- | abs => sorry
-  -- | app => sorry
-  -- | eq hA ha hb IA Ia Ib => exact ⟨.eq IA.left Ia.left Ib.left, .eq IA.right (Ia.left.cast IA) sorry⟩
-  -- | eq_rfl => sorry
-  -- | β_abs => sorry
-  -- | η_abs => sorry
-  -- | jeq_ext => sorry
-  -- | u0_ext => sorry
-  -- | u0_irr => sorry
-  -- | dne => sorry
-  -- | aoc => sorry
-  -- | symm => sorry
-  -- | cast => sorry
-  -- | trans => sorry
-  -- | _ =>
-  --   (try casesm* _ ∧ _)
-  --   constructor
-  --   · constructor <;> assumption
-  --   · constructor <;> assumption
+theorem HasTy.wk (hΔ : Ok Δ) (w : Γ ⊆ Δ) (h : Γ ⊢ a : A) : Δ ⊢ a : A
+  := by induction h generalizing Δ with
+  | var _ hx => exact .var hΔ (w hx)
+  | cast h ha Ia => exact (Ia hΔ w).cast (h.wk hΔ w)
+  | _ => constructor
+    <;> intros
+    <;> (repeat first
+    | assumption
+    | apply HasTy.ok_var
+    | apply Finset.insert_subset_insert
+    | apply_assumption)
 
--- inductive CtxOk : Finset FVar → Prop
---   | nil_ok : CtxOk ∅
---   | cons_ok {Γ i A} (hΓ : CtxOk Γ) (hA : Γ ⊢ A : .univ n) : CtxOk (insert ⟨i, A⟩ Γ)
+-- inductive Ext : Finset FVar → Finset FVar → Prop
+--   | emp (hΓ : Ok Γ) : Ext Γ ∅
+--   | cons (hΓ : Ext Γ Δ) (hA : (Γ ∪ Δ) ⊢ A ≡ A : .univ n) : Ext Γ (insert ⟨i, A⟩ Δ)
 
--- attribute [simp] CtxOk.nil_ok
+-- theorem Ext.left (hΓ : Ext Γ Δ) : Ok Γ := by induction hΓ <;> assumption
 
--- theorem CtxOk.jeq_nil {Γ} (hΓ : CtxOk Γ) : Γ ⊢ .nil : ⊤ := by induction hΓ with
---   | nil_ok => exact .nil_ok
---   | cons_ok hΓ hA => exact .cons_ok hA
+-- theorem Ext.ok (h : Ext Γ Δ) : Ok (Γ ∪ Δ) := by induction h with
+--   | emp hΓ => rw [Finset.union_empty]; exact hΓ
+--   | cons hΓ hA => rw [Finset.union_insert]; exact hA.ok_var _
 
--- theorem CtxOk.of_jeq_nil {Γ} (hΓ : Γ ⊢ .nil : ⊤) : CtxOk Γ := by
---   generalize ht : (⊤ : Term) = t at hΓ
---   generalize hn : Term.nil = n at hΓ
---   sorry
+-- theorem Ext.right (h : Ext ∅ Δ) : Ok Δ := by convert h.ok; rw [Finset.empty_union]
 
--- theorem CtxOk.iff_jeq_nil {Γ} : CtxOk Γ ↔ Γ ⊢ .nil : ⊤ := by induction Γ using Finset.induction with
---   | empty => simp
---   | insert hx Ih =>
---     rename_i x Γ
---     cases x with | mk i A =>
+-- theorem JEq.ext_singleton (i) (h : Γ ⊢ A ≡ A : .univ n) : Ext Γ {⟨i, A⟩}
+--   := .cons (.emp h.ok) (by convert h; simp)
+
+-- theorem Ext.jeq (hΔ : Ext Γ Δ) (h : Γ ⊢ a ≡ b : A) : (Γ ∪ Δ) ⊢ a ≡ b : A
+--   := by induction h generalizing Δ with
+--   | top_emp => simp [hΔ.right]
+--   | top_cons hA I => convert hΔ.ok; simp
+--   | var hΓ hx IΓ => exact .var (IΓ hΔ) (by simp [hx])
+--   | trans hab hbc Iab Ibc => exact .trans (Iab hΔ) (Ibc hΔ)
+--   | symm hab I => exact .symm (I hΔ)
+--   | pi hA L hB IA IB =>
+--     simp only [Finset.insert_union] at *
 --     constructor
---     · intro hΓ
---       sorry
---     · sorry
-
--- theorem JEq.left_wf (h : Γ ⊢ a ≡ b : A) : Γ ⊢ a : A := .trans h (.symm h)
-
--- theorem JEq.right_wf (h : Γ ⊢ a ≡ b : A) : Γ ⊢ b : A := .trans (.symm h) h
-
--- theorem JEq.cons_ok' (x : FVar) (hA : Γ ⊢ x.ty : .univ n) : (insert x Γ) ok
---   := by cases x; exact .cons_ok hA
-
--- theorem JEq.u0_jeq (hA : Γ ⊢ A : .univ 0) (hp : Γ ⊢ p : A) (hq : Γ ⊢ q : A) : Γ ⊢ p ≡ q : A
---   := .trans (.u0_irr hA hp) (.symm (.u0_irr hA hq))
-
-
--- def IsTy (Γ : Finset FVar) (A : Term) := ∃n, Γ ⊢ A : .univ n
-
--- notation Γ " ⊢ " A " isty" => IsTy Γ A
-
--- theorem IsTy.top {Γ : Finset FVar} (h : Γ ok) : Γ ⊢ .top isty := ⟨0, .top h⟩
-
--- theorem IsTy.bot {Γ : Finset FVar} (h : Γ ok) : Γ ⊢ .bot isty := ⟨0, .bot h⟩
-
--- theorem IsTy.univ {n} {Γ : Finset FVar} (h : Γ ok) : Γ ⊢ .univ n isty := ⟨n + 1, .univ h⟩
-
--- theorem IsTy.pi {Γ : Finset FVar} {A B}
---    (hA : Γ ⊢ A isty)
---    (hx : ⟨i, A⟩ ∉ Γ ∪ fv B)
---    (hB : insert ⟨i, A⟩ Γ ⊢ b0 (.free i A) • B isty)
---   : Γ ⊢ .pi A B isty
---   := have ⟨_, hA⟩ := hA; have ⟨_, hB⟩ := hB; ⟨_, .pi hA hx hB⟩
-
--- @[match_pattern]
--- theorem IsTy.eq {Γ : Finset FVar} {A a b} (hA : Γ ⊢ A isty) (ha : Γ ⊢ a : A) (hb : Γ ⊢ b : A)
---   : Γ ⊢ .eq A a b isty := have ⟨_, hA⟩ := hA; ⟨0, .eq hA ha hb⟩
-
--- theorem JEq.regular (h : Γ ⊢ a ≡ b : A) : Γ ⊢ A isty := by induction h with
---   | nil_ok => exact .top .nil_ok
---   | cons_ok hA => exact .top (.cons_ok hA)
---   | _ => sorry
-
--- -- TODO: existential introduction rules
-
--- -- TODO: universal elimination rules (?)
-
--- -- TODO: lore about universes, regularity, and other such nonsense
-
--- abbrev Wf (Γ : Finset FVar) (A : Term) := {t : Term // Γ ⊢ t : A}
-
--- instance Wf.setoid (Γ : Finset FVar) (A : Term) : Setoid (Term.Wf Γ A) where
---   r s t := Γ ⊢ s.val ≡ t.val : A
---   iseqv := {
---     refl x := x.prop,
---     symm h := .symm h,
---     trans h h' := .trans h h'
---   }
-
--- -- TODO: constructors for Wf
-
--- -- TODO: congruence theorems for Wf
-
--- abbrev Eqv (Γ : Finset FVar) (A : Term) := Quotient (Wf.setoid Γ A)
-
--- TODO: constructors for Eqv
+--     apply_assumption; assumption
+--     intros i hi
+--     apply IB
+--     assumption
+--     sorry
+--   | _ => constructor <;> apply_assumption; assumption
